Veil/Core/Tools/ModelChecker/Simulation/Result.lean
@@ -3,55 +3,17 @@ import Veil.Core.Tools.ModelChecker.Simulation.Basic
 namespace Veil.ModelChecker.Simulation
 open Lean
 
-private def earlyTerminationReasonToJson (reason : EarlyTerminationReason Unit) : Json :=
-  match reason with
-  | .foundViolatingState _ violates => Json.mkObj [
-      ("kind", "found_violating_state"),
-      ("state_fingerprint", Json.null),
-      ("violates", toJson violates)
-    ]
-  | .deadlockOccurred _ => Json.mkObj [
-      ("kind", "deadlock_occurred"),
-      ("state_fingerprint", Json.null)
-    ]
-  | .assertionFailed _ exId => Json.mkObj [
-      ("kind", "assertion_failed"),
-      ("state_fingerprint", Json.null),
-      ("exception_id", toJson exId)
-    ]
-  | .reachedDepthBound depth => Json.mkObj [
-      ("kind", "reached_depth_bound"),
-      ("depth", toJson depth)
-    ]
-  | .reachedTraceLimit maxTraces => Json.mkObj [
-      ("kind", "reached_trace_limit"),
-      ("max_traces", toJson maxTraces)
-    ]
-  | .cancelled => Json.mkObj [("kind", "cancelled")]
-
-private def terminationReasonToJson (reason : TerminationReason Unit) : Json :=
-  match reason with
-  | .exploredAllReachableStates => Json.mkObj [("kind", "explored_all_reachable_states")]
-  | .earlyTermination condition => Json.mkObj [
-      ("kind", "early_termination"),
-      ("condition", earlyTerminationReasonToJson condition)
-    ]
-
 private def resultToJson {ρ σ κ : Type} [ToJson ρ] [ToJson σ] [ToJson κ]
-  (result : ModelCheckingResult ρ σ κ Unit) : Json :=
+  (result : Option (SimulationResult ρ σ κ)) : Json :=
   match result with
-  | .foundViolation _ violation trace => Json.mkObj
+  | some (.foundViolation violation trace) => Json.mkObj
       [ ("result", "found_violation")
       , ("violation", toJson violation)
       , ("trace", toJson trace)
       , ("state_fingerprint", Json.null)
       ]
-  | .noViolationFound exploredStates reason => Json.mkObj
-      [ ("result", "no_violation_found")
-      , ("explored_states", toJson exploredStates)
-      , ("termination_reason", terminationReasonToJson reason)
-      ]
-  | .cancelled => Json.mkObj [("result", "cancelled")]
+  | some .cancelled => Json.mkObj [("result", "cancelled")]
+  | none => Json.mkObj [("result", "no_violation_found")]
 
 instance instToJsonSimulateResult {ρ σ κ : Type} [ToJson ρ] [ToJson σ] [ToJson κ] : ToJson (SimulateResult ρ σ κ) where
   toJson r := Json.mkObj [
